wip

fairness/heap_lang/simulation_adequacy.v
@@ -6,50 +6,57 @@ From trillium.fairness.heap_lang Require Export lang heap_lang_defs.
 
 Definition heap_lang_extrace : Type := extrace heap_lang.
 
+
 Section adequacy.
-(* Context . *)
-(* Context .  *)
 
-(* Let eGS := @heap_fairnessGS EM.  *)
+  Definition wp_premise
+    `{EM: ExecutionModel heap_lang M}
+    (Σ: gFunctors)
+    (s: stuckness) (e1 : expr) σ1 (s1: mstate M)
+    (R: execution_trace heap_lang → auxiliary_trace M → Prop)
+    (p: em_init_param)
+    := 
+    (∀ `{Hinv : @heapGS Σ M EM} ,
+        ⊢ (([∗ map] l ↦ v ∈ heap σ1, mapsto l (DfracOwn 1) v) ∗
+             em_init_resource s1 p (em_GS0 := heap_fairnessGS)
+           ={⊤}=∗
+              WP e1 @ s; locale_of [] e1; ⊤ {{ _, em_thread_post 0%nat (em_GS0 := heap_fairnessGS)}} ∗
+                                            rel_always_holds0 R s state_interp (fun _ => em_thread_post 0%nat (em_GS0 := heap_fairnessGS)) e1 σ1 s1)). 
 
-Theorem strong_simulation_adequacy_general
+
+  Theorem strong_simulation_adequacy_general
     `{hPre: @heapGpreS Σ M EM} (s: stuckness) (e1 : expr) σ1 (s1: M)
     (R: execution_trace heap_lang → auxiliary_trace M → Prop)
     (p: em_init_param)
-  :
-  rel_finitary R →
-  em_is_init_st ([e1], σ1) s1 ->
-  em_valid_state_evolution_fairness {tr[ ([e1], σ1) ]} {tr[ s1 ]} ->
-  (∀ `{Hinv : @heapGS Σ M EM} ,
-    ⊢ (([∗ map] l ↦ v ∈ heap σ1, mapsto l (DfracOwn 1) v) ∗
-       em_init_resource s1 p (em_GS0 := heap_fairnessGS)
-       ={⊤}=∗
-       WP e1 @ s; locale_of [] e1; ⊤ {{ _, em_thread_post 0%nat (em_GS0 := heap_fairnessGS)}} ∗
-       rel_always_holds0 R s state_interp (fun _ => em_thread_post 0%nat (em_GS0 := heap_fairnessGS)) e1 σ1 s1)) ->
-  continued_simulation R (trace_singleton ([e1], σ1)) (trace_singleton s1).
-Proof.
-  intros Hfin INIT VALID1 H.
+    :
+    rel_finitary R →
+    em_is_init_st ([e1], σ1) s1 ->
+    em_valid_state_evolution_fairness {tr[ ([e1], σ1) ]} {tr[ s1 ]} ->
+    (wp_premise Σ s e1 σ1 s1 R p) ->
+    continued_simulation R (trace_singleton ([e1], σ1)) (trace_singleton s1).
+  Proof.
+    intros Hfin INIT VALID1 H.
 
-  (* apply (wp_strong_adequacy heap_lang M Σ s); first by eauto. *)
-  intros. apply (wp_strong_adequacy heap_lang M Σ s); [done| ]. 
-  iIntros (?) "".
+    (* apply (wp_strong_adequacy heap_lang M Σ s); first by eauto. *)
+    intros. apply (wp_strong_adequacy heap_lang M Σ s); [done| ]. 
+    iIntros (?) "".
 
-  iMod (gen_heap_init (heap σ1)) as (genheap)" [Hgen [Hσ _]]".  
-  (* iMod (init_fairnessGS_LM _ _ s1 e1) as (fGS) "GEN".    *)
-  iMod (em_initialization _ s1 ([e1], σ1)) as (fGS) "[LM_INIT MSI]"; [done| ].
-  Unshelve. 2: by apply hPre. 
+    iMod (gen_heap_init (heap σ1)) as (genheap)" [Hgen [Hσ _]]".  
+    (* iMod (init_fairnessGS_LM _ _ s1 e1) as (fGS) "GEN".    *)
+    iMod (em_initialization _ s1 ([e1], σ1) p) as (fGS) "[LM_INIT MSI]"; [done| ].
+    Unshelve. 2: by apply hPre. 
 
-  set (distG := {| heap_fairnessGS := (fGS: (em_GS Σ (ExecutionModel := EM))) |}).
-  (* iMod (H distG) as "Hwp". clear H. *)
-  iPoseProof (H distG) as "Hwp". clear H.
- 
-  iExists state_interp, (fun _ => em_thread_post 0%nat), fork_post.
-  iSplitR.
-  { unfold config_wp. iIntros "!>!>" (???????) "?". done. }
+    set (distG := {| heap_fairnessGS := (fGS: (em_GS Σ (ExecutionModel := EM))) |}).
+    (* iMod (H distG) as "Hwp". clear H. *)
+    iPoseProof (H distG) as "Hwp". clear H.
+    
+    iExists state_interp, (fun _ => em_thread_post 0%nat), fork_post.
+    iSplitR.
+    { unfold config_wp. iIntros "!>!>" (???????) "?". done. }
 
-  iSpecialize ("Hwp" with "[Hσ LM_INIT]"); [by iFrame| ]. 
-  iDestruct "Hwp" as ">[Hwp H]". 
-  iModIntro. iFrame.
-Qed.
+    iSpecialize ("Hwp" with "[Hσ LM_INIT]"); [by iFrame| ]. 
+    iDestruct "Hwp" as ">[Hwp H]". 
+    iModIntro. iFrame.
+  Qed.
 
 End adequacy.
